src/CDCL/Spec.v
@@ -36,23 +36,52 @@ Lemma progress_falsified_empty : forall s s',
   progress s = Progress s' -> s'.(state_falsified) = [].
 Proof.
   intros s s' Hprogress. unfold progress in Hprogress.
-  destruct (progress_state s) as [m cm sat fals pending].
-  destruct fals as [|c fals]; [now injection Hprogress as <-|discriminate].
+  destruct s.(state_pending) as [|[l c] pending].
+  - unfold finish_progress in Hprogress.
+    destruct (progress_state s) as [m cm sat fals pending'].
+    destruct fals as [|d fals]; [now injection Hprogress as <-|discriminate].
+  - destruct (literal_value s.(state_model) l) as [[|]|] eqn:Hvalue;
+      [|discriminate|].
+    all:
+      unfold finish_progress in Hprogress.
+    all: destruct (progress_state s) as [m cm sat fals pending'].
+    all: destruct fals as [|d fals];
+      [now injection Hprogress as <-|discriminate].
 Qed.
 
 Lemma progress_conflict_spec : forall s explanation,
   progress s = Conflict explanation ->
-  exists s' c, progress_state s = s' /\
-    In c s'.(state_falsified) /\ explanation = neg c.
+  (exists s' c, progress_state s = s' /\
+    In c s'.(state_falsified) /\ explanation = neg c) \/
+  (exists l c pending, s.(state_pending) = (l, c) :: pending /\
+    literal_value s.(state_model) l = Some false /\ explanation = neg c).
 Proof.
   intros s explanation Hprogress. unfold progress in Hprogress.
-  destruct (progress_state s) as [m cm sat fals pending] eqn:Hstate.
-  destruct fals as [|c fals]; [discriminate|].
-  injection Hprogress as <-.
-  exists {| state_model := m; state_clauses := cm;
-    state_satisfied := sat; state_falsified := c :: fals;
-    state_pending := pending |}, c.
-  split; [reflexivity|]. split; [now left|reflexivity].
+  destruct s.(state_pending) as [|[l c] pending] eqn:Hpending.
+  - left. unfold finish_progress in Hprogress.
+    destruct (progress_state s) as [m cm sat fals pending'] eqn:Hstate.
+    destruct fals as [|d fals]; [discriminate|]. injection Hprogress as <-.
+    exists {| state_model := m; state_clauses := cm;
+      state_satisfied := sat; state_falsified := d :: fals;
+      state_pending := pending' |}, d. split; [reflexivity|].
+    split; [now left|reflexivity].
+  - destruct (literal_value s.(state_model) l) as [[|]|] eqn:Hvalue.
+    + left. unfold finish_progress in Hprogress.
+      destruct (progress_state s) as [m cm sat fals pending'] eqn:Hstate.
+      destruct fals as [|d fals]; [discriminate|]. injection Hprogress as <-.
+      exists {| state_model := m; state_clauses := cm;
+        state_satisfied := sat; state_falsified := d :: fals;
+        state_pending := pending' |}, d. split; [reflexivity|].
+      split; [now left|reflexivity].
+    + right. injection Hprogress as <-. exists l, c, pending.
+      repeat split; assumption.
+    + left. unfold finish_progress in Hprogress.
+      destruct (progress_state s) as [m cm sat fals pending'] eqn:Hstate.
+      destruct fals as [|d fals]; [discriminate|]. injection Hprogress as <-.
+      exists {| state_model := m; state_clauses := cm;
+        state_satisfied := sat; state_falsified := d :: fals;
+        state_pending := pending' |}, d. split; [reflexivity|].
+      split; [now left|reflexivity].
 Qed.
 
 Definition satisfies_problem (m : SModel) (p : Problem) : bool :=
@@ -113,6 +142,152 @@ Proof.
     apply (IH l); [exact Hundecided|exact Hin].
 Qed.
 
+Lemma literal_undecided_not_InL : forall m l,
+  literal_is_undecided m l = true ->
+  ~ InL (literal_var l) m.
+Proof.
+  intros m l Hundecided [Hpos|Hneg].
+  all: unfold literal_is_undecided, literal_value in Hundecided;
+       destruct (find (fun l' => literal_var l' =? literal_var l) m)
+         as [[v|v]|] eqn:Hfind.
+  all: try (destruct l; discriminate).
+  - pose proof (find_none _ _ Hfind _ Hpos) as Hfalse.
+    cbn [literal_var] in Hfalse. now rewrite Nat.eqb_refl in Hfalse.
+  - pose proof (find_none _ _ Hfind _ Hneg) as Hfalse.
+    cbn [literal_var] in Hfalse. now rewrite Nat.eqb_refl in Hfalse.
+Qed.
+
+Lemma not_InL_literal_undecided : forall m l,
+  ~ InL (literal_var l) m -> literal_is_undecided m l = true.
+Proof.
+  intros m l Hnotin. unfold literal_is_undecided, literal_value.
+  destruct (find (fun x => literal_var x =? literal_var l) m)
+    as [x|] eqn:Hfind; [|reflexivity].
+  exfalso. apply find_some in Hfind as [Hin Hvars].
+  apply Nat.eqb_eq in Hvars. apply Hnotin.
+  destruct x as [v|v]; cbn [literal_var] in Hvars; subst v;
+    [left|right]; exact Hin.
+Qed.
+
+Lemma literal_is_true_cons_undecided : forall m l x,
+  literal_is_undecided m l = true ->
+  literal_is_true m x = true ->
+  literal_is_true (l :: m) x = true.
+Proof.
+  intros m l x Hlu Hxt.
+  unfold literal_is_undecided, literal_is_true, literal_value in *.
+  simpl. destruct (literal_var l =? literal_var x) eqn:Hvars.
+  - apply Nat.eqb_eq in Hvars. rewrite Hvars in Hlu.
+    destruct (find (fun l' => literal_var l' =? literal_var x) m) eqn:Hfind.
+    + destruct l, l0; discriminate Hlu.
+    + discriminate Hxt.
+  - exact Hxt.
+Qed.
+
+Lemma literal_is_true_cons_self : forall m l,
+  literal_is_true (l :: m) l = true.
+Proof.
+  intros m [v|v]; unfold literal_is_true, literal_value; simpl;
+    rewrite Nat.eqb_refl; reflexivity.
+Qed.
+
+Lemma decided_literal_cons_undecided : forall m l x,
+  literal_is_undecided m l = true ->
+  literal_is_undecided m x = false ->
+  literal_is_true (l :: m) x = literal_is_true m x /\
+  literal_is_undecided (l :: m) x = false.
+Proof.
+  intros m l x Hlu Hxu.
+  unfold literal_is_undecided, literal_is_true, literal_value in *.
+  simpl. destruct (literal_var l =? literal_var x) eqn:Hvars.
+  - apply Nat.eqb_eq in Hvars. rewrite Hvars in Hlu.
+    destruct (find (fun l' => literal_var l' =? literal_var x) m)
+      as [y|] eqn:Hfind.
+    + destruct l, y; discriminate Hlu.
+    + discriminate Hxu.
+  - split; [reflexivity|exact Hxu].
+Qed.
+
+Lemma satisfied_cons_undecided : forall m l c,
+  literal_is_undecided m l = true ->
+  Is_true (existsb (literal_is_true m) c) ->
+  Is_true (existsb (literal_is_true (l :: m)) c).
+Proof.
+  intros m l c Hlu Hsat. apply Is_true_eq_true in Hsat.
+  apply Is_true_eq_left. apply existsb_exists in Hsat as [x [Hxc Hxt]].
+  apply existsb_exists. exists x. split; [exact Hxc|].
+  now apply literal_is_true_cons_undecided.
+Qed.
+
+Lemma falsified_cons_undecided : forall m l c,
+  literal_is_undecided m l = true ->
+  Is_true (negb (existsb (literal_is_true m) c)) /\
+    filter (literal_is_undecided m) c = [] ->
+  Is_true (negb (existsb (literal_is_true (l :: m)) c)) /\
+    filter (literal_is_undecided (l :: m)) c = [].
+Proof.
+  intros m l c Hlu. induction c as [|x xs IH]; intros [Hfalse Hdecided].
+  - now split.
+  - simpl in Hfalse, Hdecided |- *.
+    destruct (literal_is_undecided m x) eqn:Hxu; [discriminate|].
+    destruct (decided_literal_cons_undecided m l x Hlu Hxu)
+      as [Htrue Hxu'].
+    rewrite Hxu'. simpl. rewrite Htrue.
+    destruct (literal_is_true m x); simpl in Hfalse |- *.
+    + contradiction.
+    + apply IH. now split.
+Qed.
+
+Lemma InL_cons_other : forall l m v,
+  v <> literal_var l -> InL v (l :: m) -> InL v m.
+Proof.
+  intros [x|x] m v Hneq; unfold InL; simpl;
+    intros [[Heq|Hin]|[Heq|Hin]].
+  - injection Heq as ->. contradiction.
+  - now left.
+  - discriminate.
+  - now right.
+  - discriminate.
+  - now left.
+  - injection Heq as ->. contradiction.
+  - now right.
+Qed.
+
+Lemma literal_decided_cons : forall m l x,
+  literal_is_undecided m l = true ->
+  literal_is_decided m x -> literal_is_decided (l :: m) x.
+Proof.
+  intros m l x Hlu Hdecided. unfold literal_is_decided in Hdecided |- *.
+  exact (proj2 (decided_literal_cons_undecided m l x Hlu Hdecided)).
+Qed.
+
+Lemma literal_pending_cons : forall m l x,
+  literal_is_undecided m l = true ->
+  literal_is_undecided m x = true \/ literal_is_decided m x ->
+  literal_is_undecided (l :: m) x = true \/ literal_is_decided (l :: m) x.
+Proof.
+  intros m l x Hlu [Hundecided|Hdecided].
+  2:{ right. now apply literal_decided_cons. }
+  destruct (Nat.eq_dec (literal_var l) (literal_var x)) as [Heq|Hneq].
+  - right. destruct l as [v|v], x as [w|w]; cbn in Heq; subst w;
+      unfold literal_is_decided, literal_is_undecided, literal_value;
+      simpl; rewrite Nat.eqb_refl; reflexivity.
+  - left. unfold literal_is_undecided, literal_value in Hundecided |- *.
+    simpl. apply Nat.eqb_neq in Hneq. now rewrite Hneq.
+Qed.
+
+Lemma count_occ_nodup_in : forall (xs : list Clause) c,
+  NoDup xs -> In c xs -> count_occ clause_eq_dec xs c = 1.
+Proof.
+  intros xs c Hnodup. induction Hnodup as [|x xs Hnotin Hnodup IH];
+    intros Hin; [contradiction|].
+  simpl in Hin |- *. destruct Hin as [->|Hin].
+  - destruct (clause_eq_dec c c); [|contradiction].
+    rewrite (proj1 (count_occ_not_In clause_eq_dec xs c) Hnotin). reflexivity.
+  - destruct (clause_eq_dec x c) as [->|Hneq]; [contradiction|].
+    exact (IH Hin).
+Qed.
+
 (* A queued reason represents the second watch of its unit clause. *)
 Definition card_of_watch (work : list Clause) (c : Clause) (s : State) :=
   ClauseMap.card_of c s.(state_clauses).
@@ -130,14 +305,17 @@ Definition staged_invariant (work : list Clause) (s : State) : Prop :=
   /\ (forall l c, In (l, c) s.(state_pending) ->
      In l c /\
        (literal_is_undecided s.(state_model) l = true \/
-        In l s.(state_model)))
+        literal_is_decided s.(state_model) l))
+  /\ (forall c, In c work ->
+     card_of_watch work c s = 1 \/
+     (card_of_watch work c s = 0 /\
+       exists l, In (l, c) s.(state_pending)))
   /\ (forall c,
      card_of_watch work c s = 0 \/
      card_of_watch work c s = 2 \/
      (card_of_watch work c s = 1 /\
        (In c work \/ exists l,
-         In (l, c) s.(state_pending) /\
-         literal_is_undecided s.(state_model) l = true))).
+         In (l, c) s.(state_pending)))).
 
 Definition state_invariant (s : State) : Prop := staged_invariant [] s.
 
@@ -156,10 +334,597 @@ Proof.
         -- intros v. rewrite ClauseMap.find_empty. constructor.
         -- split; [constructor|]. split.
            ++ intros l c H. contradiction.
-           ++ intros c. unfold card_of_watch, pending_clauses.
-              cbn [state_clauses state_pending].
-              rewrite ClauseMap.card_of_empty. now left.
+           ++ split.
+              ** intros c H. contradiction.
+              ** intros c. unfold card_of_watch, pending_clauses.
+                 cbn [state_clauses state_pending].
+                 rewrite ClauseMap.card_of_empty. now left.
 Qed.
 
-(* Lemma progress_state_inv : forall s s', *)
-(*     state_invariant s -> progress s = Progress s' -> state_invariant s'. *)
+Lemma scan_clause_once_spec : forall m c,
+  scan_clause_once m c =
+    (existsb (literal_is_true m) c, filter (literal_is_undecided m) c).
+Proof.
+  intros m c. induction c as [|l c IH]; simpl; [reflexivity|].
+  now rewrite IH.
+Qed.
+
+Lemma find_different_var_spec : forall v ls l,
+  find_different_var v ls = Some l ->
+  In l ls /\ v <> literal_var l.
+Proof.
+  intros v ls. induction ls as [|x xs IH]; intros l Hfind; simpl in Hfind.
+  - discriminate.
+  - destruct (v =? literal_var x) eqn:Heq.
+    + destruct (IH l Hfind) as [Hin Hneq]. now split; [right|].
+    + injection Hfind as ->. split; [now left|].
+      now apply Nat.eqb_neq.
+Qed.
+
+Lemma scan_clause_inl_spec : forall m c cm sat fals l,
+  scan_clause m c cm sat fals = propagate_literal l ->
+  In l c /\ literal_is_undecided m l = true.
+Proof.
+  intros m c cm sat fals l Hscan. unfold scan_clause in Hscan.
+  rewrite scan_clause_once_spec in Hscan.
+  destruct (existsb (literal_is_true m) c); [discriminate|].
+  destruct (filter (literal_is_undecided m) c) as [|x xs]
+    eqn:Hfilter; [discriminate|].
+  destruct (find_different_var (literal_var x) xs).
+  - destruct (in_dec clause_eq_dec c (ClauseMap.find (literal_var x) cm));
+      discriminate.
+  - injection Hscan as <-.
+  assert (In x (filter (literal_is_undecided m) c)) as Hin.
+  { rewrite Hfilter. now left. }
+  now apply filter_In in Hin.
+Qed.
+
+Lemma scan_clause_watched_spec : forall m c cm sat fals cm',
+  scan_clause m c cm sat fals = clause_watched cm' ->
+  exists l l', existsb (literal_is_true m) c = false /\
+    In l c /\ In l' c /\
+    literal_is_undecided m l = true /\
+    literal_is_undecided m l' = true /\
+    literal_var l <> literal_var l' /\
+    cm' = if in_dec clause_eq_dec c (ClauseMap.find (literal_var l) cm)
+      then ClauseMap.add (literal_var l') c cm
+      else ClauseMap.add (literal_var l) c cm.
+Proof.
+  intros m c cm sat fals cm' Hscan. unfold scan_clause in Hscan.
+  rewrite scan_clause_once_spec in Hscan.
+  destruct (existsb (literal_is_true m) c); [discriminate|].
+  destruct (filter (literal_is_undecided m) c) as [|l undecided]
+    eqn:Hfilter; [discriminate|].
+  destruct (find_different_var (literal_var l) undecided) as [l'|]
+    eqn:Hdifferent; [|discriminate].
+  apply find_different_var_spec in Hdifferent as [Hl'in Hneq].
+  assert (In l (filter (literal_is_undecided m) c)) as Hlin
+    by (rewrite Hfilter; now left).
+  assert (In l' (filter (literal_is_undecided m) c)) as Hl'in'.
+  { rewrite Hfilter. now right. }
+  apply filter_In in Hlin as [Hlc Hlu].
+  apply filter_In in Hl'in' as [Hl'c Hl'u].
+  exists l, l'. repeat split; try assumption.
+  destruct (in_dec clause_eq_dec c (ClauseMap.find (literal_var l) cm));
+    now injection Hscan as <-.
+Qed.
+
+Lemma scan_clause_decided_spec : forall m c cm sat fals cm' sat' fals',
+  scan_clause m c cm sat fals = clause_decided cm' sat' fals' ->
+  (existsb (literal_is_true m) c = true /\
+    cm' = ClauseMap.remove_clause c cm /\ sat' = c :: sat /\ fals' = fals) \/
+  (existsb (literal_is_true m) c = false /\
+    filter (literal_is_undecided m) c = [] /\
+    cm' = ClauseMap.remove_clause c cm /\ sat' = sat /\ fals' = c :: fals).
+Proof.
+  intros m c cm sat fals cm' sat' fals' Hscan. unfold scan_clause in Hscan.
+  rewrite scan_clause_once_spec in Hscan.
+  destruct (existsb (literal_is_true m) c) eqn:Htrue.
+  - injection Hscan as <- <- <-. now left.
+  - destruct (filter (literal_is_undecided m) c) as [|l undecided]
+      eqn:Hfilter.
+    + injection Hscan as <- <- <-. right. repeat split; assumption.
+    + destruct (find_different_var (literal_var l) undecided) as [l'|].
+      * destruct (in_dec clause_eq_dec c
+          (ClauseMap.find (literal_var l) cm)); discriminate.
+      * discriminate.
+Qed.
+
+Lemma watch_one_fresh_inv : forall work m cm sat fals pending c l,
+  staged_invariant (c :: work)
+    {| state_model := m; state_clauses := cm;
+       state_satisfied := sat; state_falsified := fals;
+       state_pending := pending |} ->
+  existsb (literal_is_true m) c = false ->
+  ~ In c (ClauseMap.find (literal_var l) cm) ->
+  In l c -> literal_is_undecided m l = true ->
+  staged_invariant work
+    {| state_model := m; state_clauses := ClauseMap.add (literal_var l) c cm;
+       state_satisfied := sat; state_falsified := fals;
+       state_pending := pending |}.
+Proof.
+  intros work m cm sat fals pending c l Hinv Hfalse Hfresh Hlc Hlu.
+  destruct Hinv as
+    [Hsat [Hfals [Hwatch [Hnodup [Hworknodup
+      [Hpending [Hwork Hcard]]]]]]].
+  inversion Hworknodup as [|? ? Hcnotin Hworknodup']; subst.
+  pose proof (Hwork c (or_introl eq_refl)) as Hcwork.
+  unfold card_of_watch in Hcwork. cbn -[ClauseMap.card_of] in Hcwork.
+  split; [exact Hsat|]. split; [exact Hfals|]. split.
+  - intros v d Hin. apply ClauseMap.find_add in Hin as [[-> ->]|Hin].
+    + split; [now apply literal_undecided_not_InL|now apply literal_InL].
+    + now apply Hwatch with (c := d).
+  - split.
+    + intros v. cbn [state_clauses]. rewrite ClauseMap.find_add_eq.
+      destruct (VarKey.eq_dec (literal_var l) v) as [Heq|Hneq].
+      * subst v. constructor; [exact Hfresh|apply Hnodup].
+      * apply Hnodup.
+    + split; [exact Hworknodup'|]. split; [exact Hpending|]. split.
+      * intros d Hdwork. specialize (Hwork d (or_intror Hdwork)).
+        assert (c <> d) as Hcd.
+        { intros ->. contradiction. }
+        unfold card_of_watch in Hwork |- *.
+        cbn -[ClauseMap.card_of] in Hwork |- *.
+        rewrite (ClauseMap.card_of_add_neq cm c d (literal_var l) Hcd).
+        exact Hwork.
+      * intros d. destruct (clause_eq_dec c d) as [->|Hcd].
+        -- unfold card_of_watch. cbn -[ClauseMap.card_of].
+           rewrite ClauseMap.card_of_add.
+           destruct Hcwork as [Hone|[Hzero [p Hpc]]].
+           ++ rewrite Hone. now right; left.
+           ++ rewrite Hzero. right; right. split; [reflexivity|].
+              right. now exists p.
+        -- specialize (Hcard d).
+           unfold card_of_watch in Hcard |- *.
+           cbn -[ClauseMap.card_of] in Hcard |- *.
+           rewrite (ClauseMap.card_of_add_neq cm c d (literal_var l) Hcd).
+           destruct Hcard as [Hzero|[Htwo|[Hone Hreason]]].
+           ++ now left.
+           ++ now right; left.
+           ++ right; right. split; [exact Hone|].
+              destruct Hreason as [Hdwork|Hpendingreason].
+              ** simpl in Hdwork. destruct Hdwork as [Heq|Hdwork];
+                   [contradiction|now left].
+              ** now right.
+Qed.
+
+Lemma watch_one_inv : forall work m cm sat fals pending c l l' cm',
+  staged_invariant (c :: work)
+    {| state_model := m; state_clauses := cm;
+       state_satisfied := sat; state_falsified := fals;
+       state_pending := pending |} ->
+  existsb (literal_is_true m) c = false ->
+  In l c -> In l' c ->
+  literal_is_undecided m l = true ->
+  literal_is_undecided m l' = true ->
+  literal_var l <> literal_var l' ->
+  cm' = (if in_dec clause_eq_dec c (ClauseMap.find (literal_var l) cm)
+    then ClauseMap.add (literal_var l') c cm
+    else ClauseMap.add (literal_var l) c cm) ->
+  staged_invariant work
+    {| state_model := m; state_clauses := cm';
+       state_satisfied := sat; state_falsified := fals;
+       state_pending := pending |}.
+Proof.
+  intros work m cm sat fals pending c l l' cm' Hinv Hfalse
+    Hlc Hl'c Hlu Hl'u Hneq Hcm'.
+  destruct (in_dec clause_eq_dec c (ClauseMap.find (literal_var l) cm))
+    as [Hwatched|Hfresh].
+  - subst cm'. apply watch_one_fresh_inv; try assumption.
+    intros Hwatched'.
+    destruct Hinv as [_ [_ [_ [_ [_ [_ [Hwork _]]]]]]].
+    specialize (Hwork c (or_introl eq_refl)).
+    unfold card_of_watch in Hwork. cbn -[ClauseMap.card_of] in Hwork.
+    assert (ClauseMap.card_of c cm = 1) as Hcone.
+    { destruct Hwork as [Hone|[Hzero _]]; [exact Hone|].
+      pose proof (ClauseMap.card_of_in cm c (literal_var l) Hwatched).
+      lia. }
+    apply Hneq. eapply ClauseMap.card_of_unique; eauto.
+  - subst cm'. now apply watch_one_fresh_inv.
+Qed.
+
+Lemma propagate_literal_inv : forall work m cm sat fals pending c l,
+  staged_invariant (c :: work)
+    {| state_model := m; state_clauses := cm;
+       state_satisfied := sat; state_falsified := fals;
+       state_pending := pending |} ->
+  scan_clause m c cm sat fals = propagate_literal l ->
+  staged_invariant work
+    {| state_model := m; state_clauses := cm;
+       state_satisfied := sat; state_falsified := fals;
+       state_pending := (l, c) :: pending |}.
+Proof.
+  intros work m cm sat fals pending c l Hinv Hscan.
+  pose proof (scan_clause_inl_spec _ _ _ _ _ _ Hscan) as [Hlc Hlu].
+  destruct Hinv as
+    [Hsat [Hfals [Hwatch [Hnodup [Hworknodup
+      [Hpending [Hwork Hcard]]]]]]].
+  inversion Hworknodup as [|? ? Hcnotin Hworknodup']; subst.
+  split; [exact Hsat|]. split; [exact Hfals|]. split; [exact Hwatch|].
+  split; [exact Hnodup|]. split; [exact Hworknodup'|]. split.
+  - intros p d Hpd. simpl in Hpd. destruct Hpd as [Heq|Hpd].
+    + injection Heq as <- <-. split; [exact Hlc|now left].
+    + exact (Hpending p d Hpd).
+  - split.
+    + intros d Hdwork. specialize (Hwork d (or_intror Hdwork)).
+      destruct Hwork as [Hone|[Hzero [p Hpd]]].
+      * now left.
+      * right. split; [exact Hzero|]. exists p. now right.
+    + intros d. specialize (Hcard d).
+      destruct Hcard as [Hzero|[Htwo|[Hone Hreason]]].
+      * now left.
+      * now right; left.
+      * right; right. split; [exact Hone|].
+        destruct Hreason as [Hdwork|[p Hpd]].
+        -- simpl in Hdwork. destruct Hdwork as [->|Hdwork].
+           ++ right. exists l. now left.
+           ++ now left.
+        -- right. exists p. now right.
+Qed.
+
+Lemma remove_active_inv : forall work m cm sat fals pending c sat' fals',
+  staged_invariant (c :: work)
+    {| state_model := m; state_clauses := cm;
+       state_satisfied := sat; state_falsified := fals;
+       state_pending := pending |} ->
+  (forall d, In d sat' -> Is_true (existsb (literal_is_true m) d)) ->
+  (forall d, In d fals' ->
+    Is_true (negb (existsb (literal_is_true m) d)) /\
+    filter (literal_is_undecided m) d = []) ->
+  staged_invariant work
+    {| state_model := m; state_clauses := ClauseMap.remove_clause c cm;
+       state_satisfied := sat'; state_falsified := fals';
+       state_pending := pending |}.
+Proof.
+  intros work m cm sat fals pending c sat' fals' Hinv Hsat' Hfals'.
+  destruct Hinv as
+    [_ [_ [Hwatch [Hnodup [Hworknodup
+      [Hpending [Hwork Hcard]]]]]]].
+  inversion Hworknodup as [|? ? Hcnotin Hworknodup']; subst.
+  split; [exact Hsat'|]. split; [exact Hfals'|]. split.
+  - intros v d Hin. apply ClauseMap.find_remove_clause in Hin as [Hin _].
+    exact (Hwatch v d Hin).
+  - split.
+    + intros v. cbn [state_clauses]. rewrite ClauseMap.find_remove_clause_eq.
+      apply NoDup_filter. apply Hnodup.
+    + split; [exact Hworknodup'|]. split; [exact Hpending|]. split.
+      * intros d Hdwork. assert (c <> d) as Hcd by (intros ->; contradiction).
+        specialize (Hwork d (or_intror Hdwork)).
+        unfold card_of_watch in Hwork |- *.
+        cbn -[ClauseMap.card_of] in Hwork |- *.
+        rewrite (ClauseMap.card_of_remove_clause_neq cm c d Hcd).
+        exact Hwork.
+      * intros d. destruct (clause_eq_dec c d) as [->|Hcd].
+        -- unfold card_of_watch. cbn -[ClauseMap.card_of].
+           rewrite ClauseMap.card_of_remove_clause_eq. now left.
+        -- specialize (Hcard d).
+           unfold card_of_watch in Hcard |- *.
+           cbn -[ClauseMap.card_of] in Hcard |- *.
+           rewrite (ClauseMap.card_of_remove_clause_neq cm c d Hcd).
+           destruct Hcard as [Hzero|[Htwo|[Hone Hreason]]].
+           ++ now left.
+           ++ now right; left.
+           ++ right; right. split; [exact Hone|].
+              destruct Hreason as [Hdwork|Hpendingreason].
+              ** simpl in Hdwork. destruct Hdwork as [Heq|Hdwork];
+                   [contradiction|now left].
+              ** now right.
+Qed.
+
+Lemma propagate_decided_inv : forall work m cm sat fals pending c cm' sat' fals',
+  staged_invariant (c :: work)
+    {| state_model := m; state_clauses := cm;
+       state_satisfied := sat; state_falsified := fals;
+       state_pending := pending |} ->
+  scan_clause m c cm sat fals = clause_decided cm' sat' fals' ->
+  staged_invariant work
+    {| state_model := m; state_clauses := cm';
+       state_satisfied := sat'; state_falsified := fals';
+       state_pending := pending |}.
+Proof.
+  intros work m cm sat fals pending c cm' sat' fals' Hinv Hscan.
+  pose proof (scan_clause_decided_spec _ _ _ _ _ _ _ _ Hscan) as Hspec.
+  pose proof Hinv as Hinv'.
+  destruct Hinv as [Hsat [Hfals Hrest]].
+  destruct Hspec as [[Htrue [-> [-> ->]]]|[Hfalse [Hfilter [-> [-> ->]]]]].
+  - eapply remove_active_inv.
+    + exact Hinv'.
+    + intros d Hd. simpl in Hd. destruct Hd as [->|Hd];
+        [now rewrite Htrue|exact (Hsat d Hd)].
+    + exact Hfals.
+  - eapply remove_active_inv.
+    + exact Hinv'.
+    + exact Hsat.
+    + intros d Hd. simpl in Hd. destruct Hd as [->|Hd].
+      * split; [now rewrite Hfalse|exact Hfilter].
+      * exact (Hfals d Hd).
+Qed.
+
+Lemma propagate_inv : forall c work s,
+  staged_invariant (c :: work) s ->
+  staged_invariant work (propagate c s).
+Proof.
+  intros c work [m cm sat fals pending] Hinv.
+  unfold propagate. cbn [state_model state_clauses state_satisfied
+    state_falsified state_pending] in Hinv |- *.
+  destruct (scan_clause m c cm sat fals) as [l|cm' sat' fals'|cm']
+    eqn:Hscan.
+  - now eapply propagate_literal_inv.
+  - eapply propagate_decided_inv.
+    + exact Hinv.
+    + exact Hscan.
+  - pose proof (scan_clause_watched_spec _ _ _ _ _ _ Hscan) as
+      [l [l' [Hfalse [Hlc [Hl'c [Hlu [Hl'u [Hneq Hcm']]]]]]]].
+    eapply watch_one_inv.
+    + exact Hinv.
+    + exact Hfalse.
+    + exact Hlc.
+    + exact Hl'c.
+    + exact Hlu.
+    + exact Hl'u.
+    + exact Hneq.
+    + exact Hcm'.
+Qed.
+
+Lemma prepare_set_lit_inv : forall l m cm sat fals pending,
+  literal_is_undecided m l = true ->
+  state_invariant
+    {| state_model := m; state_clauses := cm;
+       state_satisfied := sat; state_falsified := fals;
+       state_pending := pending |} ->
+  staged_invariant (ClauseMap.find (literal_var l) cm)
+    {| state_model := l :: m;
+       state_clauses := ClauseMap.remove (literal_var l) cm;
+       state_satisfied := sat; state_falsified := fals;
+       state_pending := pending |}.
+Proof.
+  intros l m cm sat fals pending Hlu Hinv.
+  destruct Hinv as
+    [Hsat [Hfals [Hwatch [Hnodup [_ [Hpending [_ Hcard]]]]]]].
+  split.
+  - intros c Hin. apply satisfied_cons_undecided; [exact Hlu|exact (Hsat c Hin)].
+  - split.
+    + intros c Hin. apply falsified_cons_undecided; [exact Hlu|exact (Hfals c Hin)].
+    + split.
+      * intros v c Hin. apply ClauseMap.find_remove in Hin as [Hin Hneq].
+        destruct (Hwatch v c Hin) as [Hnotin Hinc]. split; [|exact Hinc].
+        intros Hinmodel. apply Hnotin.
+        eapply InL_cons_other; [exact Hneq|exact Hinmodel].
+      * split.
+        -- intros v. cbn [state_clauses]. rewrite ClauseMap.find_remove_eq.
+           destruct (VarKey.eq_dec (literal_var l) v);
+             [constructor|apply Hnodup].
+        -- split; [apply Hnodup|]. split.
+           ++ intros p c Hpc. destruct (Hpending p c Hpc) as [Hpin Hp].
+              split; [exact Hpin|now apply literal_pending_cons].
+           ++ split.
+              ** intros c Hcin.
+                 pose proof (ClauseMap.card_of_in cm c (literal_var l) Hcin)
+                   as Hpos.
+                 pose proof (ClauseMap.card_of_remove cm c (literal_var l))
+                   as Hremove.
+                 change (ClauseMap.card_of c (ClauseMap.remove (literal_var l) cm) +
+                   count_occ clause_eq_dec (ClauseMap.find (literal_var l) cm) c =
+                   ClauseMap.card_of c cm) in Hremove.
+                 pose proof (count_occ_nodup_in
+                   (ClauseMap.find (literal_var l) cm) c
+                   (Hnodup (literal_var l)) Hcin) as Hcount.
+                 specialize (Hcard c).
+                 unfold card_of_watch in Hcard |- *.
+                 cbn -[ClauseMap.card_of] in Hcard |- *.
+                 destruct Hcard as [Hzero|[Htwo|[Hone Hreason]]].
+                 --- lia.
+                 --- left. rewrite Hcount, Htwo in Hremove. lia.
+                 --- right. split; [rewrite Hcount, Hone in Hremove; lia|].
+                     destruct Hreason as [Habs|[p Hpc]];
+                       [contradiction|now exists p].
+              ** intros c.
+                 pose proof (ClauseMap.card_of_remove cm c (literal_var l))
+                   as Hremove.
+                 change (ClauseMap.card_of c (ClauseMap.remove (literal_var l) cm) +
+                   count_occ clause_eq_dec (ClauseMap.find (literal_var l) cm) c =
+                   ClauseMap.card_of c cm) in Hremove.
+                 specialize (Hcard c).
+                 unfold card_of_watch in Hcard |- *.
+                 cbn -[ClauseMap.card_of] in Hcard |- *.
+                 destruct (in_dec clause_eq_dec c
+                   (ClauseMap.find (literal_var l) cm)) as [Hcin|Hnotin].
+                 --- pose proof (count_occ_nodup_in
+                       (ClauseMap.find (literal_var l) cm) c
+                       (Hnodup (literal_var l)) Hcin) as Hcount.
+                     destruct Hcard as [Hzero|[Htwo|[Hone Hreason]]].
+                     +++ left. lia.
+                     +++ right; right. split.
+                         *** rewrite Hcount, Htwo in Hremove. lia.
+                         *** now left.
+                     +++ left. rewrite Hcount, Hone in Hremove. lia.
+                 --- pose proof (proj1 (count_occ_not_In clause_eq_dec
+                       (ClauseMap.find (literal_var l) cm) c) Hnotin) as Hcount.
+                     destruct Hcard as [Hzero|[Htwo|[Hone Hreason]]].
+                     +++ left. lia.
+                     +++ right; left. rewrite Hcount, Htwo in Hremove. lia.
+                     +++ right; right. split.
+                         *** rewrite Hcount, Hone in Hremove. lia.
+                         ***
+                         destruct Hreason as [Habs|Hpendingreason];
+                           [contradiction|now right].
+Qed.
+
+Lemma fold_propagate_inv : forall work s,
+  staged_invariant work s ->
+  state_invariant (fold_left (fun s c => propagate c s) work s).
+Proof.
+  induction work as [|c work IH]; intros s Hinv; [exact Hinv|].
+  simpl. apply IH. now apply propagate_inv.
+Qed.
+
+Lemma set_lit_inv : forall l s,
+  literal_is_undecided s.(state_model) l = true ->
+  state_invariant s -> state_invariant (set_lit l s).
+Proof.
+  intros l [m cm sat fals pending] Hlu Hinv.
+  unfold set_lit. cbn [state_model state_clauses state_satisfied
+    state_falsified state_pending].
+  apply fold_propagate_inv.
+  now apply prepare_set_lit_inv.
+Qed.
+
+Lemma remove_pending_inv : forall l c pending m cm sat fals,
+  state_invariant
+    {| state_model := m; state_clauses := cm;
+       state_satisfied := sat; state_falsified := fals;
+       state_pending := (l, c) :: pending |} ->
+  state_invariant
+    {| state_model := m; state_clauses := ClauseMap.remove_clause c cm;
+       state_satisfied := sat; state_falsified := fals;
+       state_pending := pending |}.
+Proof.
+  intros l c pending m cm sat fals Hinv.
+  destruct Hinv as
+    [Hsat [Hfals [Hwatch [Hnodup [_ [Hpending [_ Hcard]]]]]]].
+  split; [exact Hsat|]. split; [exact Hfals|]. split.
+  - intros v d Hin. apply ClauseMap.find_remove_clause in Hin as [Hin _].
+    exact (Hwatch v d Hin).
+  - split.
+    + intros v. cbn [state_clauses]. rewrite ClauseMap.find_remove_clause_eq.
+      apply NoDup_filter. apply Hnodup.
+    + split; [constructor|]. split.
+      * intros p d Hpd. exact (Hpending p d (or_intror Hpd)).
+      * split; [intros d Habs; contradiction|]. intros d.
+        destruct (clause_eq_dec c d) as [->|Hcd].
+        -- unfold card_of_watch. cbn -[ClauseMap.card_of].
+           rewrite ClauseMap.card_of_remove_clause_eq. now left.
+        -- specialize (Hcard d).
+           unfold card_of_watch in Hcard |- *.
+           cbn -[ClauseMap.card_of] in Hcard |- *.
+           rewrite (ClauseMap.card_of_remove_clause_neq cm c d Hcd).
+           destruct Hcard as [Hzero|[Htwo|[Hone [Habs|[p Hpd]]]]].
+           ++ now left.
+           ++ now right; left.
+           ++ contradiction.
+           ++ right; right. split; [exact Hone|]. right. exists p.
+              simpl in Hpd. destruct Hpd as [Heq|Hpd]; [congruence|exact Hpd].
+Qed.
+
+Lemma staged_add_satisfied : forall work s c,
+  staged_invariant work s ->
+  Is_true (existsb (literal_is_true s.(state_model)) c) ->
+  staged_invariant work
+    {| state_model := s.(state_model); state_clauses := s.(state_clauses);
+       state_satisfied := c :: s.(state_satisfied);
+       state_falsified := s.(state_falsified);
+       state_pending := s.(state_pending) |}.
+Proof.
+  intros work [m cm sat fals pending] c Hinv Htrue.
+  destruct Hinv as [Hsat Hrest]. split; [|exact Hrest].
+  intros d Hd. simpl in Hd. destruct Hd as [->|Hd]; [exact Htrue|exact (Hsat d Hd)].
+Qed.
+
+Lemma set_pending_inv : forall l c pending m cm sat fals,
+  literal_is_undecided m l = true ->
+  state_invariant
+    {| state_model := m; state_clauses := cm;
+       state_satisfied := sat; state_falsified := fals;
+       state_pending := (l, c) :: pending |} ->
+  state_invariant
+    (set_lit l
+      {| state_model := m; state_clauses := ClauseMap.remove_clause c cm;
+         state_satisfied := c :: sat; state_falsified := fals;
+         state_pending := pending |}).
+Proof.
+  intros l c pending m cm sat fals Hlu Hinv.
+  pose proof Hinv as Hpendinginv.
+  destruct Hpendinginv as [_ [_ [_ [_ [_ [Hpending _]]]]]].
+  destruct (Hpending l c (or_introl eq_refl)) as [Hlc _].
+  pose proof (remove_pending_inv l c pending m cm sat fals Hinv) as Hremoved.
+  unfold set_lit. cbn [state_model state_clauses state_satisfied
+    state_falsified state_pending].
+  apply fold_propagate_inv.
+  pose proof (prepare_set_lit_inv l m (ClauseMap.remove_clause c cm)
+    sat fals pending Hlu Hremoved) as Hprepared.
+  destruct Hprepared as [Hsat Hrest]. split; [|exact Hrest].
+  intros d Hd. simpl in Hd. destruct Hd as [->|Hd].
+  - apply Is_true_eq_left. apply existsb_exists. exists l.
+    split; [exact Hlc|apply literal_is_true_cons_self].
+  - exact (Hsat d Hd).
+Qed.
+
+Lemma resolve_true_pending_inv : forall l c pending m cm sat fals,
+  literal_is_true m l = true ->
+  state_invariant
+    {| state_model := m; state_clauses := cm;
+       state_satisfied := sat; state_falsified := fals;
+       state_pending := (l, c) :: pending |} ->
+  state_invariant
+    {| state_model := m; state_clauses := ClauseMap.remove_clause c cm;
+       state_satisfied := c :: sat; state_falsified := fals;
+       state_pending := pending |}.
+Proof.
+  intros l c pending m cm sat fals Hltrue Hinv.
+  pose proof Hinv as Hpendinginv.
+  destruct Hpendinginv as [_ [_ [_ [_ [_ [Hpending _]]]]]].
+  destruct (Hpending l c (or_introl eq_refl)) as [Hlc _].
+  pose proof (remove_pending_inv l c pending m cm sat fals Hinv) as Hremoved.
+  destruct Hremoved as [Hsat Hrest]. split; [|exact Hrest].
+  intros d Hd. simpl in Hd. destruct Hd as [->|Hd].
+  - apply Is_true_eq_left. apply existsb_exists. now exists l.
+  - exact (Hsat d Hd).
+Qed.
+
+Lemma finish_progress_inv : forall s s',
+  state_invariant s -> finish_progress s = Progress s' -> state_invariant s'.
+Proof.
+  intros [m cm sat fals pending] s' Hinv Hfinish.
+  unfold finish_progress in Hfinish. destruct fals as [|c fals];
+    [now injection Hfinish as <-|discriminate].
+Qed.
+
+Lemma progress_inv : forall s s',
+  state_invariant s -> progress s = Progress s' -> state_invariant s'.
+Proof.
+  intros [m cm sat fals pending] s' Hinv Hprogress.
+  unfold progress in Hprogress.
+  cbn [state_pending state_model] in Hprogress.
+  destruct pending as [|[l c] pending].
+  - apply finish_progress_inv with
+      (s := progress_state
+        {| state_model := m; state_clauses := cm;
+           state_satisfied := sat; state_falsified := fals;
+           state_pending := [] |}); [|exact Hprogress].
+    unfold progress_state. cbn [state_pending state_model state_clauses
+      state_satisfied state_falsified].
+    destruct (hd_error (ClauseMap.keys cm)) as [v|] eqn:Hhead.
+    + apply set_lit_inv; [|exact Hinv].
+      apply not_InL_literal_undecided.
+      assert (In v (ClauseMap.keys cm)) as Hkey.
+      { destruct (ClauseMap.keys cm) as [|x xs] eqn:Hkeys;
+          [discriminate|]. injection Hhead as <-. now left. }
+      apply <- ClauseMap.keys_complete in Hkey.
+      destruct (ClauseMap.find v cm) as [|d ds] eqn:Hfind;
+        [contradiction|].
+      destruct Hinv as [_ [_ [Hwatch _]]].
+      assert (In d (ClauseMap.find v cm)) as Hin by (rewrite Hfind; now left).
+      exact (proj1 (Hwatch v d Hin)).
+    + exact Hinv.
+  - destruct (literal_value m l) as [[|]|] eqn:Hvalue.
+    + apply finish_progress_inv with
+        (s := progress_state
+          {| state_model := m; state_clauses := cm;
+             state_satisfied := sat; state_falsified := fals;
+             state_pending := (l, c) :: pending |}); [|exact Hprogress].
+      unfold progress_state. cbn [state_pending state_model state_clauses
+        state_satisfied state_falsified]. rewrite Hvalue.
+      apply (resolve_true_pending_inv l c pending m cm sat fals);
+        [|exact Hinv].
+      unfold literal_is_true. now rewrite Hvalue.
+    + discriminate.
+    + apply finish_progress_inv with
+        (s := progress_state
+          {| state_model := m; state_clauses := cm;
+             state_satisfied := sat; state_falsified := fals;
+             state_pending := (l, c) :: pending |}); [|exact Hprogress].
+      unfold progress_state. cbn [state_pending state_model state_clauses
+        state_satisfied state_falsified]. rewrite Hvalue.
+      apply (set_pending_inv l c pending m cm sat fals); [|exact Hinv].
+      unfold literal_is_undecided. now rewrite Hvalue.
+Qed.
